src/DY.Example.NSL.Protocol.Total.fst
@@ -12,9 +12,6 @@ open DY.Lib
 //
 // [2] Gavin Lowe. "Breaking and fixing the Needham-Schroeder Public-Key
 //     Protocol using FDR". TACAS, pp 147-166, 1996.
-//
-// Note: the version implemented in DY* has a modified msg 3:
-// it is {N_B, A}K_PB
 
 val (let?): #a:Type -> #b:Type -> x:option a -> (y:a -> Pure (option b) (requires x == Some y) (ensures fun _ -> True)) -> option b
 let (let?) #a #b x f =
@@ -48,8 +45,6 @@ type message2_ (bytes:Type0) {|bytes_like bytes|} = {
 
 type message3_ (bytes:Type0) {|bytes_like bytes|} = {
   n_b: bytes;
-  // The `alice` principal is an addition of DY* example
-  alice: principal;
 }
 
 %splice [ps_message3_] (gen_parser (`message3_))
@@ -103,7 +98,7 @@ let decode_message2 alice bob msg2_cipher sk_a n_a =
 
 val compute_message3: principal -> principal -> bytes -> bytes -> bytes -> bytes
 let compute_message3 alice bob pk_b n_b nonce =
-  let msg3 = Msg3 {n_b; alice;} in
+  let msg3 = Msg3 {n_b;} in
   pk_enc pk_b nonce (serialize message msg3)
 
 val decode_message3: principal -> principal -> bytes -> bytes -> bytes -> option (message3)
@@ -113,5 +108,4 @@ let decode_message3 alice bob msg_cipher sk_b n_b =
   guard (Msg3? msg);?
   let (Msg3 msg3) = msg in
   guard (n_b = msg3.n_b);?
-  guard (alice = msg3.alice);?
   Some msg3
